\documentclass{article}
\usepackage[english]{babel}
\usepackage{amsmath,amssymb}

%%%%%%%%%% Start TeXmacs macros
\newcommand{\tmaffiliation}[1]{\\ #1}
\newcommand{\tmop}[1]{\ensuremath{\operatorname{#1}}}
%%%%%%%%%% End TeXmacs macros

\begin{document}


\begin{center}
  $f (x) = \sum^{\infty}_{n = 0} \cos (x + n \pi)$

\end{center}

\begin{center}
  $= \sum^{\infty}_{n = 0} \tmop{Re} [e^{^{i (x + n \pi)}}]$

\end{center}

\begin{center}
 $= \tmop{Re} \left[ \sum^{\infty}_{n = 0} e^{^{i (x + n \pi)}} \right]$

\end{center}

\begin{center}
 = $\tmop{Re} \left[ e^{^{ix}} \sum^{\infty}_{n = 0} (e^{^{in \pi}})
  \right]$.

\end{center}

\begin{center}
$\sum^{\infty}_{n = 0} (e^{^{in \pi}}) = 1 / 1 - e^{^{i \pi}} = 1 / 2.$

\end{center}

\begin{center}
  $\tmop{Re} \left[ e^{^{ix}} \sum^{\infty}_{n = 0} (e^{^{in \pi}}) \right]$

\end{center}
  
\begin{center}
  $= \tmop{Re} [e^{^{ix}} / 2]$

\end{center}

\begin{center}  
  $=^{^{}} \cos (x) / 2.$

\end{center}

\begin{center}
  $f (x) = \sum^{\infty}_{n = 0} \cos (x + n \pi) =^{^{}} \cos (x) / 2.$

\end{center}

\begin{center}
  $f (0) = \sum^{\infty}_{n = 0} \cos (n \pi) = 1 - 1 + 1 - 1 + \cdot \cdot
  \cdot = \sum^{\infty}_{n = 0} (- 1)^{^n} = \cos (0) / 2 = 1 / 2.$

\end{center}

\begin{center}
  $\sum^{\infty}_{n = 0} (- 1)^{^n} = 1 / 2.$

\end{center}

\end{document}